Import (partial) rework using dependent types

tlc/comp/slc.v
@@ -1,206 +1,137 @@
 From mathcomp.ssreflect
 Require Import ssreflect eqtype ssrbool ssrfun seq.
+From tlc.utility
+Require Import indeq hseq.
 From tlc.assert
-Require Import all_assert.
-
-Require Import comp flc.
+Require Import scope type rigid_var term atom prop lib.
+From tlc.comp
+Require Import component flc.
 
 Set Implicit Arguments.
 Unset Strict Implicit.
 Unset Printing Implicit Defensive.
 
+(* Stubborn link component *)
 Section slc.
 
-  Variable node : eqType.
-  Variable message : eqType.
+  Variable N : eqType. (* Node type *)
+  Variable M : eqType. (* Message type *)
 
-  (* Concrete requests *)
-  Inductive req_sl_ : Type :=
-  | Send_sl : node -> message -> req_sl_.
+  (* Requests *)
+  Section req.
 
-  (* Equality *)
-  Section req_sl__eq.
+    Inductive req_sl_ : Type :=
+    | Send_sl : N -> M -> req_sl_.
 
-    Definition eq_req_sl_ (r r' : req_sl_) :=
-      match r, r' with
-      | Send_sl n m, Send_sl n' m' => (n == n') && (m == m')
-      end.
+    (* Equality *)
+    Section eq.
 
-    Lemma eq_req_sl_P : Equality.axiom eq_req_sl_.
-    Proof.
-      case=> [n m]; case=> [n' m'];
-        rewrite /eq_req_sl_ /=; try by constructor.
-      - (* Send_sl *)
-        case Hn: (n == n');
-          [move/eqP: Hn => ?; subst n' | constructor];
-          last by case=> ?; subst n'; rewrite eqxx in Hn.
-        case Hm: (m == m');
-          [move/eqP: Hm => ?; subst m' | constructor];
-          last by case=> ?; subst m'; rewrite eqxx in Hm.
-        by constructor.
-    Qed.
+      Definition eq_req_sl_ (e e' : req_sl_) :=
+        match e, e' with
+        | Send_sl n m, Send_sl n' m' => (n == n') && (m == m')
+        end.
 
-    Canonical req_sl__eqMixin :=
-      Eval hnf in EqMixin eq_req_sl_P.
-    Canonical req_sl__eqType :=
-      Eval hnf in EqType req_sl_ req_sl__eqMixin.
+      Lemma eq_req_sl_P : Equality.axiom eq_req_sl_.
+      Proof.
+        case=> [n m]; case=> [n' m']; indeq_auto.
+        - (* Send_sl *) indeq n n'; indeq m m'; by [].
+      Qed.
+
+      Canonical req_sl__eqMixin :=
+        Eval hnf in EqMixin eq_req_sl_P.
+      Canonical req_sl__eqType :=
+        Eval hnf in EqType req_sl_ req_sl__eqMixin.
+
+    End eq.
 
     Definition req_sl := [eqType of req_sl_].
 
-  End req_sl__eq.
+  End req.
 
-  (* Assertion requests *)
-  Inductive req_sl_A_ : Type :=
-  | Send_sl_A : node_variable -> message_variable -> req_sl_A_.
+  (* Indications *)
+  Section ind.
 
-  (* Equality *)
-  Section req_sl_A__eq.
+    Inductive ind_sl_ : Type :=
+    | Deliver_sl : N -> M -> ind_sl_.
 
-    Definition eq_req_sl_A_ (r r' : req_sl_A_) :=
-      match r, r' with
-      | Send_sl_A n m, Send_sl_A n' m' => (n == n') && (m == m')
-      end.
+    (* Equality *)
+    Section eq.
 
-    Lemma eq_req_sl_A_P : Equality.axiom eq_req_sl_A_.
-    Proof.
-      case=> [n m]; case=> [n' m'];
-        rewrite /eq_req_sl_A_ /=; try by constructor.
-      - (* Send_sl_A *)
-        case Hn: (n == n');
-          [move/eqP: Hn => ?; subst n' | constructor];
-          last by case=> ?; subst n'; rewrite eqxx in Hn.
-        case Hm: (m == m');
-          [move/eqP: Hm => ?; subst m' | constructor];
-          last by case=> ?; subst m'; rewrite eqxx in Hm.
-        by constructor.
-    Qed.
+      Definition eq_ind_sl_ (e e' : ind_sl_) :=
+        match e, e' with
+        | Deliver_sl n m, Deliver_sl n' m' => (n == n') && (m == m')
+        end.
 
-    Canonical req_sl_A__eqMixin :=
-      Eval hnf in EqMixin eq_req_sl_A_P.
-    Canonical req_sl_A__eqType :=
-      Eval hnf in EqType req_sl_A_ req_sl_A__eqMixin.
+      Lemma eq_ind_sl_P : Equality.axiom eq_ind_sl_.
+      Proof.
+        case=> [n m]; case=> [n' m']; indeq_auto.
+        - (* Deliver_sl *) indeq n n'; indeq m m'; by [].
+      Qed.
 
-    Definition req_sl_A := [eqType of req_sl_A_].
+      Canonical ind_sl__eqMixin :=
+        Eval hnf in EqMixin eq_ind_sl_P.
+      Canonical ind_sl__eqType :=
+        Eval hnf in EqType ind_sl_ ind_sl__eqMixin.
 
-  End req_sl_A__eq.
-
-  (* Concrete indications *)
-  Inductive ind_sl_ : Type :=
-  | Deliver_sl : node -> message -> ind_sl_.
-
-  (* Equality *)
-  Section ind_sl__eq.
-
-    Definition eq_ind_sl_ (r r' : ind_sl_) :=
-      match r, r' with
-      | Deliver_sl n m, Deliver_sl n' m' => (n == n') && (m == m')
-      end.
-
-    Lemma eq_ind_sl_P : Equality.axiom eq_ind_sl_.
-    Proof.
-      case=> [n m]; case=> [n' m'];
-        rewrite /eq_ind_sl_ /=; try by constructor.
-      - (* Deliver_sl *)
-        case Hn: (n == n');
-          [move/eqP: Hn => ?; subst n' | constructor];
-          last by case=> ?; subst n'; rewrite eqxx in Hn.
-        case Hm: (m == m');
-          [move/eqP: Hm => ?; subst m' | constructor];
-          last by case=> ?; subst m'; rewrite eqxx in Hm.
-        by constructor.
-    Qed.
-
-    Canonical ind_sl__eqMixin :=
-      Eval hnf in EqMixin eq_ind_sl_P.
-    Canonical ind_sl__eqType :=
-      Eval hnf in EqType ind_sl_ ind_sl__eqMixin.
+    End eq.
 
     Definition ind_sl := [eqType of ind_sl_].
 
-  End ind_sl__eq.
-
-  (* Assertion indications *)
-  Inductive ind_sl_A_ : Type :=
-  | Deliver_sl_A : node_variable -> message_variable -> ind_sl_A_.
-
-  (* Equality *)
-  Section ind_sl_A__eq.
-
-    Definition eq_ind_sl_A_ (r r' : ind_sl_A_) :=
-      match r, r' with
-      | Deliver_sl_A n m, Deliver_sl_A n' m' => (n == n') && (m == m')
-      end.
-
-    Lemma eq_ind_sl_A_P : Equality.axiom eq_ind_sl_A_.
-    Proof.
-      case=> [n m]; case=> [n' m'];
-        rewrite /eq_ind_sl_A_ /=; try by constructor.
-      - (* Deliver_sl_A *)
-        case Hn: (n == n');
-          [move/eqP: Hn => ?; subst n' | constructor];
-          last by case=> ?; subst n'; rewrite eqxx in Hn.
-        case Hm: (m == m');
-          [move/eqP: Hm => ?; subst m' | constructor];
-          last by case=> ?; subst m'; rewrite eqxx in Hm.
-        by constructor.
-    Qed.
-
-    Canonical ind_sl_A__eqMixin :=
-      Eval hnf in EqMixin eq_ind_sl_A_P.
-    Canonical ind_sl_A__eqType :=
-      Eval hnf in EqType ind_sl_A_ ind_sl_A__eqMixin.
-
-    Definition ind_sl_A := [eqType of ind_sl_A_].
-
-  End ind_sl_A__eq.
+  End ind.
 
   (* State *)
-  Definition slc_state := seq (prod node message).
+  Definition state_sl := [eqType of seq (prod N M)].
 
   (* Component *)
-  Definition slc_subcomps :=
-    [:: Subcomp (req_fl node message)
-                (ind_fl node message)].
+  Definition sub_sl :=
+    [:: (@req_fl N M, @ind_fl N M)].
   Definition slc :=
     let flc := 0 in
-    let slc_init n := [::] in
-    let slc_request n s ir :=
+    let init_sl n := [::] in
+    let request_sl n s ir :=
       match ir with
       | Send_sl n' m =>
         ((n', m) :: s, [:: Send_fl n' m], [::])
       end in
-    let slc_indication n' s ii :=
+    let indication_sl n' s ii :=
       match ii with
       | Deliver_fl n m =>
         (s, [::], [:: Deliver_sl n m])
       end in
-    let slc_periodic n s :=
+    let periodic_sl n s :=
       let ors := [seq Send_fl p.1 p.2 | p <- s] in
       (s, ors, [::]) in
-    @Comp node req_sl ind_sl slc_subcomps
-      slc_state slc_init
-      slc_request slc_indication slc_periodic.
-
-  (* Specification *)
-  Section spec.
-
-    Import AssertNotations.
-
-    Local Notation Vrn' := (first_node_var).
-
-    (* Non-compiling
-    (* SL_1: Stubborn delivery *)
-    Definition SL_1 :=
-      ((Pcorrect?(Vrn)) /\ (Pcorrect?(Vrn')) ->
-      (on: Vrn, ev: [], Creq_ev, (Send_sl_A Vrn' Vrm) =>
-       alwaysf: eventf: on: Vrn', ev: [], Cind_ev, (Deliver_sl_A Vrn Vrm)))%A.
-
-    (* SL_2: No-forge *)
-    Definition SL_2 :=
-      (on: Vrn, ev: [], Cind_ev, (Deliver_sl_A Vrn' Vrm) <~
-      on: Vrn', ev: [], Creq_ev, (Send_sl_A Vrn Vrm))%A.
-    *)
-
-  End spec.
+    @Component N M req_sl ind_sl sub_sl
+      state_sl init_sl request_sl indication_sl periodic_sl.
 
 End slc.
+
+(* Specification of SLC *)
+Module SLCSpec.
+
+Import TLC.
+
+(* Constructors for events *)
+Definition Send_sl {N M} :=
+  @Const (slc N M) (Node -> Message -> IREvent) (@Send_sl N M).
+Definition Deliver_sl {N M} :=
+  @Const (slc N M) (Node -> Message -> OIEvent) (@Deliver_sl N M).
+
+Local Notation n' := (RigidVar Node 0).
+Local Notation m := (RigidVar Message 0).
+
+(* SL_1: Stubborn delivery *)
+Definition SL_1 {N M}
+: @prop (slc N M) :=
+  Atom (correct <- Fn) /\ Atom (correct <- n') ->
+  (on: Fn, ev: [], Request, EventIR <- (Send_sl <- n' <- m)) =>:
+  (alwaysf: existsf: on: n', ev: [], Indication,
+    EventOI <- (Deliver_sl <- Fn <- m)).
+
+(* SL_2: No-forge *)
+Definition SL_2 {N M}
+: @prop (slc N M) :=
+  on: Fn, ev: [], Indication, EventOI <- (Deliver_sl <- n' <- m) <~
+  on: n', ev: [], Request, EventIR <- (Send_sl <- Fn <- m).
+
+End SLCSpec.
