tlc/utility/variant.v
@@ -1,16 +1,68 @@
 From mathcomp.ssreflect
-Require Import ssreflect eqtype ssrbool seq.
+Require Import ssreflect eqtype ssrbool seq ssrnat fintype.
+From tlc.utility
+Require Import seq lemmas.
 
 Set Implicit Arguments.
 Unset Strict Implicit.
 Unset Printing Implicit Defensive.
 
-Section variant.
+(* Right-associative sum types parameterized by sequences of types *)
 
-  Fixpoint variant (types : seq Type) : Type :=
-    match types with
-    | nil => unit
-    | x :: t => if t is nil then x else sum x (variant t)
-    end.
+Fixpoint variant (ts : seq Type) : Type :=
+  match ts with
+  | nil => unit
+  | t :: nil => t
+  | t :: ts' => sum t (variant ts')
+  end.
 
-End variant.
+Fixpoint eqVariant (ts : seq eqType) : eqType :=
+  match ts with
+  | nil => [eqType of unit]
+  | t :: nil => t
+  | t :: ts' => [eqType of sum t (eqVariant ts')]
+  end.
+
+Lemma variant_cons (t : Type) (ts : seq Type) :
+  ts <> nil ->
+  sum t (variant ts) = variant (t :: ts).
+Proof.
+  move=> H. case H': ts; last by [].
+  by contradiction.
+Qed.
+
+Lemma eqVariant_cons (t : eqType) (ts : seq eqType) :
+  ts <> nil ->
+  [eqType of sum t (eqVariant ts)] = eqVariant (t :: ts).
+Proof.
+  move=> H. case H': ts; last by [].
+  by contradiction.
+Qed.
+
+Fixpoint ini (ts : seq Type) (i : 'I_(size ts)) : ith i -> variant ts.
+  case: ts i => [ | t ts] [i H];
+  rewrite /nat_of_ord => x //;
+  case Hts: ts => [ | t' ts'].
+  - (* ts = [::] *)
+    subst ts.
+    assert (H' := H); move: H'; rewrite ltnS leqn0 /=; move/eqP=> Hi; subst i.
+    move: x; rewrite //.
+  - (* ts = t' :: ts' *)
+    case Hi: i => [ | i']; subst i; first by apply (inl x).
+    rewrite -variant_cons; last by [].
+    rewrite -Hts; exact: (inr (ini ts _ x)).
+Defined.
+
+Fixpoint eq_ini (ts : seq eqType) (i : 'I_(size ts)) : ith i -> eqVariant ts.
+  case: ts i => [ | t ts] [i H];
+  rewrite /nat_of_ord => x //;
+  case Hts: ts => [ | t' ts'].
+  - (* ts = [::] *)
+    subst ts.
+    assert (H' := H); move: H'; rewrite ltnS leqn0 /=; move/eqP=> Hi; subst i.
+    move: x; rewrite //.
+  - (* ts = t' :: ts' *)
+    case Hi: i => [ | i']; subst i; first by apply (inl x).
+    rewrite -eqVariant_cons; last by [].
+    rewrite -Hts; exact: (inr (eq_ini ts _ x)).
+Defined.
