tlc/all/all.v
@@ -1,4 +1,0 @@
-Require Export tlc.assert.all_assert.
-Require Export tlc.comp.all_comp.
-Require Export tlc.logic.all_logic.
-Require Export tlc.utility.all_utility.
