tlc/assert/constant_prop.v
@@ -1,0 +1,32 @@
+From mathcomp.ssreflect
+Require Import ssreflect.
+From tlc.assert
+Require Import rigid_var atom prop interleavable_prop.
+
+Set Implicit Arguments.
+Unset Strict Implicit.
+Unset Printing Implicit Defensive.
+
+Inductive constant_prop {C} : @prop C -> Type :=
+| CAAtom a :
+  constant_prop (Atom a)
+| CAConj A1 A2 :
+  constant_prop A1 ->
+  constant_prop A2 ->
+  constant_prop (Conj A1 A2)
+| CANeg A0 :
+  constant_prop A0 ->
+  constant_prop (Neg A0)
+| CAAlways t (x : rigid_var t) A0 :
+  constant_prop A0 ->
+  constant_prop (Always x A0).
+
+Definition constant_prop_t {C} :=
+  {A : @prop C & constant_prop A}.
+
+Lemma constant_prop_is_interleavable {C} A
+  (CA : @constant_prop C A) :
+  interleavable_prop A.
+Proof.
+  elim: CA; by constructor.
+Qed.
