tlc/assert/depth_inv.v
@@ -1,0 +1,13 @@
+From mathcomp.ssreflect
+Require Import ssreflect ssrnat seq.
+From tlc.assert
+Require Import prop interleavable_prop depth_prop.
+
+Set Implicit Arguments.
+Unset Strict Implicit.
+Unset Printing Implicit Defensive.
+
+Inductive depth_inv {C} (d : seq nat) : @prop C -> Type :=
+| DI A :
+  depth_prop d A ->
+  depth_inv d (AlwaysF A).
