tlc/assert/depth_prop.v
@@ -1,0 +1,47 @@
+From mathcomp.ssreflect
+Require Import ssreflect ssrbool ssrnat seq.
+From tlc.utility
+Require Import seq.
+From tlc.assert
+Require Import type rigid_var term atom prop lib interleavable_prop.
+
+Set Implicit Arguments.
+Unset Strict Implicit.
+Unset Printing Implicit Defensive.
+
+Inductive depth_prop {C} (d : seq nat) : @prop C -> Type :=
+| DACorrect t :
+  depth_prop d (Atom (App TLC.correct t))
+| DAEv n d' o e :
+  d' <<< d ->
+  depth_prop d (TLC.On n (TLC.Ev (@seq_to_term C Nat d') o e))
+| DAConj A1 A2 :
+  depth_prop d A1 ->
+  depth_prop d A2 ->
+  depth_prop d (Conj A1 A2)
+| DANeg A0 :
+  depth_prop d A0 ->
+  depth_prop d (Neg A0)
+| DAAlways t (x : rigid_var t) A0 :
+  depth_prop d A0 ->
+  depth_prop d (Always x A0)
+| DAAlwaysF' A0 :
+  depth_prop d A0 ->
+  depth_prop d (AlwaysF' A0)
+| DAAlwaysP' A0 :
+  depth_prop d A0 ->
+  depth_prop d (AlwaysP' A0)
+| DAExistsF' A0 :
+  depth_prop d A0 ->
+  depth_prop d (ExistsF' A0)
+| DAExistsP' A0 :
+  depth_prop d A0 ->
+  depth_prop d (ExistsP' A0).
+
+Lemma depth_prop_is_interleavable {C} d A
+  (DA : @depth_prop C d A) :
+  interleavable_prop A.
+Proof.
+  elim: DA; try by constructor;
+  try by (rewrite /TLC.On /TLC.Ev /TLC.Eq; repeat constructor).
+Qed.
