tlc/assert/flexible_var.v
@@ -1,0 +1,62 @@
+From mathcomp.ssreflect
+Require Import ssreflect eqtype ssrbool.
+From tlc.utility
+Require Import indeq.
+From tlc.assert
+Require Import type.
+
+Set Implicit Arguments.
+Unset Strict Implicit.
+Unset Printing Implicit Defensive.
+
+(* Named flexible variables in the assertion language *)
+Inductive flexible_var : Type :=
+| Fn
+| Fd
+| Fo
+| Fe
+| Fors
+| Fois
+| Fs
+| Fs'.
+
+(* Equality *)
+Section eq.
+
+  Definition flexible_var_eq (x x' : flexible_var) :=
+    match x, x' with
+    | Fn, Fn => true
+    | Fd, Fd => true
+    | Fo, Fo => true
+    | Fe, Fe => true
+    | Fors, Fors => true
+    | Fois, Fois => true
+    | Fs, Fs => true
+    | Fs', Fs' => true
+    | _, _ => false
+    end.
+
+  Lemma flexible_var_eqP : Equality.axiom flexible_var_eq.
+  Proof.
+    case; case; by indeq_auto.
+  Qed.
+
+  Canonical flexible_var_eqMixin :=
+    EqMixin flexible_var_eqP.
+  Canonical flexible_var_eqType :=
+    Eval hnf in EqType flexible_var flexible_var_eqMixin.
+
+End eq.
+
+(* Maps flexible variables to their types *)
+Definition type_flexible_var {C} x : @type C :=
+  match x with
+  | Fn => Node
+  | Fd => Depth
+  | Fo => Orientation
+  | Fe => Event
+  | Fors => [OREvent]
+  | Fois => [OIEvent]
+  | Fs => States
+  | Fs' => States
+  end.
