tlc/assert/interleavable_prop.v
@@ -1,0 +1,37 @@
+From mathcomp.ssreflect
+Require Import ssreflect.
+From tlc.assert
+Require Import rigid_var atom prop.
+
+Set Implicit Arguments.
+Unset Strict Implicit.
+Unset Printing Implicit Defensive.
+
+Inductive interleavable_prop {C} : @prop C -> Type :=
+| IAAtom a :
+  interleavable_prop (Atom a)
+| IAConj A1 A2 :
+  interleavable_prop A1 ->
+  interleavable_prop A2 ->
+  interleavable_prop (Conj A1 A2)
+| IANeg A0 :
+  interleavable_prop A0 ->
+  interleavable_prop (Neg A0)
+| IAAlways t (x : rigid_var t) A0 :
+  interleavable_prop A0 ->
+  interleavable_prop (Always x A0)
+| IAAlwaysF' A0 :
+  interleavable_prop A0 ->
+  interleavable_prop (AlwaysF' A0)
+| IAAlwaysP' A0 :
+  interleavable_prop A0 ->
+  interleavable_prop (AlwaysP' A0)
+| IAExistsF' A0 :
+  interleavable_prop A0 ->
+  interleavable_prop (ExistsF' A0)
+| IAExistsP' A0 :
+  interleavable_prop A0 ->
+  interleavable_prop (ExistsP' A0).
+
+Definition interleavable_prop_t {C} :=
+  {A : @prop C & interleavable_prop A}.
