tlc/assert/lib.v
@@ -1,0 +1,365 @@
+From Coq.Lists
+Require Import List.
+From mathcomp.ssreflect
+Require Import ssreflect eqtype ssrbool ssrnat seq fintype.
+From tlc.utility
+Require Import seq variant lemmas.
+From tlc.comp
+Require Import all_comp.
+From tlc.assert
+Require Import scope orientation type flexible_var rigid_var term atom prop.
+
+Set Implicit Arguments.
+Unset Strict Implicit.
+Unset Printing Implicit Defensive.
+
+(* TODO: Placeholdes *)
+Definition correct {C} (n : node C) : bool := true.
+Definition Correct {C} : seq (node C) := [::].
+Definition Nodes {C} : seq (node C) := [::].
+
+Fixpoint denote_eq {C} t : @denote_type C (t -> t -> Bool) :=
+  let: t' := @denote_type C t in
+  match t with
+  | Unit => fun x y => true
+  | Func t1 t2 => fun x y => x == y
+  | Product t1 t2 =>
+    fun x y => (denote_eq (fst x) (fst y)) && (denote_eq (snd x) (snd y))
+  | Sum t1 t2 =>
+    fun x y =>
+      match x, y with
+      | inl x', inl y' => denote_eq x' y'
+      | inr x', inr y' => denote_eq x' y'
+      | _, _ => false
+      end
+  | List t' =>
+    fix e x y :=
+      match x, y with
+      | [::], [::] => true
+      | x1 :: s1', x2 :: s2' => denote_eq x1 x2 && e s1' s2'
+      | _, _ => false
+      end
+  | Bool => fun x y => x == y
+  | Nat => fun x y => x == y
+  | Node => fun x y => x == y
+  | Message => fun x y => x == y
+  | Orientation => fun x y => x == y
+  | IREvent => fun x y => x == y
+  | OIEvent => fun x y => x == y
+  | OREvent' _ => fun x y => x == y
+  | IIEvent' _ => fun x y => x == y
+  | PEvent => fun x y => x == y
+  | State => fun x y => x == y
+  end.
+
+Module TLC.
+
+(* Constructors for events *)
+Definition EventIR {C} :=
+  @Const C (IREvent -> Event) (fun x => inl (inl (inl (inl x)))).
+Definition EventOI {C} :=
+  @Const C (OIEvent -> Event) (fun x => inl (inl (inl (inr x)))).
+Definition EventOR {C} :=
+  @Const C (OREvent -> Event) (fun x => inl (inl (inr x))).
+Definition EventII {C} :=
+  @Const C (IIEvent -> Event) (fun x => inl (inr x)).
+Definition per {C} :=
+  @Const C Event (inr per).
+
+(* Equality of terms *)
+Section eq.
+
+  Definition eq {C t} :=
+    @Const C _ (@denote_eq C t).
+  Definition Eq {C t} (x y : @term C t) : atom :=
+    eq <- x <- y.
+
+End eq.
+
+(* Notation for term equality *)
+Notation "x = y" :=
+  (Eq x y)
+  (at level 70, no associativity) : tlc_core_scope.
+
+(* Boolean constants *)
+Section bool.
+
+  Definition true {C} := @Const C Bool true.
+  Definition false {C} := @Const C Bool false.
+
+End bool.
+
+(* Product functions *)
+Section product.
+
+  Definition pair {C t1 t2} :=
+    @Const C (t1 -> t2 -> t1 * t2) pair.
+
+End product.
+
+(* Notations for building products *)
+Notation "( x , y , .. , z )" :=
+  (pair <- (.. (pair <- x <- y) ..) <- z)%tlc
+  : tlc_core_scope.
+
+(* Sum functions *)
+Section sum.
+
+  Definition inl {C t1 t2} :=
+    @Const C (t1 -> t1 + t2) inl.
+  Definition inr {C t1 t2} :=
+    @Const C (t2 -> t1 + t2) inr.
+
+  Definition ini {C} {ts : seq (@type C)} (i : 'I_(size ts)) :
+    @term C (ith i -> Variant ts).
+    case Hts: ts i => [ | t ts'] i; case Hi: i => [n Hs];
+    case Hn: n Hs Hi => [ | n'] Hs Hi; try by [];
+    apply Const; rewrite denote_func denote_variant;
+    remember [seq denote_type t | t <- ts] as Ts;
+    have H: (size Ts = size ts) by subst Ts; exact: size_map.
+    - (* ts = t :: ts', n = 0 *)
+      assert (HeqTs' := HeqTs); rewrite Hts /= in HeqTs'.
+      have HS: (0 < size Ts) by rewrite HeqTs'.
+      rewrite HeqTs' in HS; pose I := Ordinal HS.
+      have Ht: (denote_type t = ith I) by subst I; exact: ith0.
+      rewrite ith0 Ht -Hts -HeqTs HeqTs'; exact: eq_ini.
+    - (* ts = t :: ts', n = n'.+1 *)
+      assert (HeqTs' := HeqTs); rewrite Hts /= in HeqTs'.
+      have HS: (n'.+1 < size Ts) by rewrite HeqTs /= size_map Hts //.
+      rewrite HeqTs' in HS; pose I := Ordinal HS.
+      have Ht: (denote_type (ith i) = ith I).
+        subst i I; move: HS; rewrite -map_cons => HS; exact: ith_map.
+      rewrite -Hi Ht -Hts -HeqTs HeqTs'; exact: eq_ini.
+  Unshelve. apply Ts.
+  Defined.
+
+End sum.
+
+(* List constants and functions *)
+Section list.
+
+  Definition nil {C t} :=
+    @Const C [t] nil.
+  Definition cons {C t} :=
+    @Const C (t -> [t] -> [t]) cons.
+  Definition rcons {C t} :=
+    @Const C ([t] -> t -> [t]) rcons.
+
+  Definition mem {C t} :=
+    @Const C (t -> [t] -> Bool) (fun x s => has (@denote_eq C t x) s).
+  Definition occ {C t} :=
+    @Const C (t -> [t] -> Nat) (fun x s => count (@denote_eq C t x) s).
+
+End list.
+
+(* Notations for building lists *)
+Notation "[ ]" :=
+  nil
+  : tlc_core_scope.
+Notation "[ x ]" :=
+  (cons <- x <- nil)%tlc
+  : tlc_core_scope.
+Notation "[ x ; y ; .. ; z ]" :=
+  (cons <- x <- (cons <- y <- (.. (cons <- z <- nil) ..)))%tlc
+  : tlc_core_scope.
+
+(* Natural functions *)
+Section nat.
+
+  Definition ltn {C} :=
+    @Const C (Nat -> Nat -> Bool) (fun x y => x < y).
+  Definition len {C} (x y : @term C Nat) : @prop C :=
+    Atom (ltn <- x <- y) \/ x = y.
+  Definition gtn {C} (x y : @term C Nat) : @prop C :=
+    ~(len x y).
+  Definition gen {C} (x y : @term C Nat) : @prop C :=
+    gtn x y \/ x = y.
+
+End nat.
+
+(* Notations for natural comparisons *)
+Notation "x < y" :=
+  (ltn <- x <- y)%tlc
+  : tlc_core_scope.
+Notation "x <= y" :=
+  (len x y)%tlc
+  : tlc_core_scope.
+Notation "x > y" :=
+  (gtn x y)%tlc
+  : tlc_core_scope.
+Notation "x >= y" :=
+  (gen x y)%tlc
+  : tlc_core_scope.
+
+(* Orientation constants *)
+Section orientation.
+
+  Definition Request {C} := @Const C Orientation Request.
+  Definition Indication {C} := @Const C Orientation Indication.
+  Definition Periodic {C} := @Const C Orientation Periodic.
+
+End orientation.
+
+(* Correct node classification *)
+Section correct.
+
+  (* TODO: Holes *)
+  Definition correct {C} := @Const C (Node -> Bool) correct.
+  Definition Correct {C} := @Const C [Node] Correct.
+  Definition Nodes {C} := @Const C [Node] Nodes.
+
+End correct.
+
+(* Flexible variables *)
+Section flexible.
+
+  Definition Fn {C} := @Flexible C Fn.
+  Definition Fd {C} := @Flexible C Fd.
+  Definition Fo {C} := @Flexible C Fo.
+  Definition Fe {C} := @Flexible C Fe.
+  Definition Fors {C} := @Flexible C Fors.
+  Definition Fois {C} := @Flexible C Fois.
+  Definition Fs {C} := @Flexible C Fs.
+  Definition Fs' {C} := @Flexible C Fs'.
+
+End flexible.
+
+(* Component types and functions *)
+Section component.
+
+  (* Event handler functions *)
+  Definition Output {C} : @type C := State * [OREvent] * [OIEvent].
+  Definition init {C} :=
+    @Const C (Node -> State) (@init C).
+  Definition request {C} : @term C (Node -> State -> IREvent -> Output).
+    apply Const; rewrite /= denote_or_event.
+    by exact: request.
+  Defined.
+  Definition indication {C} : @term C (Node -> State -> IIEvent -> Output).
+    apply Const; rewrite /= denote_ii_event denote_or_event.
+    by exact: indication.
+  Defined.
+  Definition periodic {C} : @term C (Node -> State -> Output).
+    apply Const; rewrite /= denote_or_event.
+    by exact: periodic.
+  Defined.
+
+End component.
+
+(* Syntactic sugar for events *)
+Section sugar.
+
+  Definition On {C} n A : @prop C :=
+    Fn = n /\ A.
+  Definition Ev {C} d o e : @prop C :=
+    Fd = d /\ Fo = o /\ Fe = e.
+  Definition SelfEv {C} : @prop C :=
+    let: request_ev := Fd = nil /\ Fo = Request in
+    let: periodic_ev := Fd = nil /\ Fo = Periodic in
+    let: indication_ev :=
+      let: i := RigidVar Nat 0 in
+      always: i, (Fd = [Rigid i] /\ Fo = Indication) in
+    request_ev \/ periodic_ev \/ indication_ev.
+
+End sugar.
+
+(* Notations for syntactic sugars *)
+Notation "'on:' n , P" :=
+  (On n P)
+  (at level 65, right associativity) : tlc_core_scope.
+Notation "'ev:' d , o , e" :=
+  (Ev d o e)
+  (at level 65, right associativity) : tlc_core_scope.
+Notation "'self'" := (SelfEv)
+  : tlc_core_scope.
+
+(* Basic program logic rules *)
+Definition PNode {C} : @prop C :=
+  alwaysf: Atom (mem <- Fn <- Nodes).
+Definition PIR {C} (e : @term C IREvent) : @prop C :=
+  ev: [], Request, EventIR <- e =>:
+  (Fs' <- Fn, Fors, Fois) = request <- Fn <- (Fs <- Fn) <- e.
+Definition PII {C} (i : 'I_(size (@IIEvents C))) (e : @term C (ith i))
+: @prop C :=
+  let: ie := @Const C Nat i in
+  let: ei := ini i <- e in
+  ev: [ie], Indication, EventII <- ei =>:
+  (Fs' <- Fn, Fors, Fois) = indication <- Fn <- (Fs <- Fn) <- ei.
+Definition PPe {C} : @prop C :=
+  ev: [], Periodic, per =>:
+  (Fs' <- Fn, Fors, Fois) = periodic <- Fn <- (Fs <- Fn).
+Definition POR {C} (n : @term C Node)
+(i : 'I_(size (@OREvents C))) (e : @term C (ith i)) : @prop C :=
+  let: ie := @Const C Nat i in
+  let: ei := ini i <- e in
+  on: n, (Atom (mem <- ei <- Fors) /\ self) =>:
+  existsf^: on: n, ev: [ie], Request, EventOR <- ei.
+Definition POI {C} (n : @term C Node) (e : @term C OIEvent) : @prop C :=
+  on: n, (Atom (mem <- e <- Fois) /\ self) =>:
+  existsf^: on: n, ev: [], Indication, EventOI <- e.
+Definition POR' {C} (n : @term C Node)
+(i : 'I_(size (@OREvents C))) (e : @term C (ith i)) : @prop C :=
+  let: ie := @Const C Nat i in
+  let: ei := ini i <- e in
+  on: n, ev: [ie], Request, EventOR <- ei =>:
+  existsp^: on: n, (Atom (mem <- ei <- Fors) /\ self).
+Definition POI' {C} (n : @term C Node) (e : @term C OIEvent) : @prop C :=
+  on: n, ev: [], Indication, EventOI <- e =>:
+  existsp^: on: n, (Atom (mem <- e <- Fois) /\ self).
+Definition PInit {C} (n : @term C Node) : @prop C :=
+  self: (Fs <- n = init <- n).
+Definition PPostPre {C} (n : @term C Node) (s : @term C State) : @prop C :=
+  self: (Atom (mem <- n <- Nodes) ->
+    (Fs' <- n = s <=>: next: (Fs <- n = s))).
+Definition PSeq {C} (n : @term C Node) : @prop C :=
+  ~(Fn = n) =>: (Fs' <- n = Fs <- n).
+Definition PASelf {C} : @prop C :=
+  self: alwaysf: self.
+(* TODO: PLSInv; need restrict *)
+Definition PCSet {C} (n : @term C Node) : @prop C :=
+  (Atom (correct <- n)) <-> (Atom (mem <- n <- Correct)).
+Definition PAPer {C} (n : @term C Node) : @prop C :=
+  (Atom (mem <- n <- Correct)) ->
+  alwaysf: existsf: on: n, ev: [], Periodic, per.
+Lemma InP (T : eqType) (x : T) (s : seq T) : reflect (In x s) (x \in s).
+  (* TODO *)
+Admitted.
+Definition PFLoss {C}
+(Hr : In req_fl (@or_events C))
+(Hi : In ind_fl (@ii_events C))
+(n n' : @term C Node) (m : @term C Message) : @prop C :=
+  let: ir := ith (findex (Hr) in
+  let: ii := ith (findex Hi) in
+  let: ie := @Const C Nat ir in
+  (Atom (correct <- n')) ->
+  alwaysf: existsf: on: n, ev: [ie], Request, (Send_fl <- n' <- m) ->
+  alwaysf: existsf: on: n', ev: [ie], Indication, (Deliver_fl <- n <- m).
+*)
+(* TODO: PLFDup; how to construct events from FLC *)
+(* TODO: PLNForge; how to construct events from FLC *)
+Definition PUniOR {C} (n : @term C Node)
+(i : 'I_(size OREvents)) (e : @term C (ith i)) : @prop C :=
+  let: ie := @Const C Nat i in
+  let: ei := ini i <- e in
+  ((occ <- ei <- Fors) <= (@Const _ Nat 1) /\
+    alwaysp^: (Fn = n /\ self -> ~(Atom (mem <- ei <- Fors))) /\
+    alwaysf^: (Fn = n /\ self -> ~(Atom (mem <- ei <- Fors)))) =>:
+  (on: n, ev: [], Indication, EventOR <- ei) =>:
+  ((alwaysp^: ~(on: n, ev: [ie], Request, EventOR <- ei)) /\
+    (alwaysf^: ~(on: n, ev: [ie], Request, EventOR <- ei))).
+Definition PUniOI {C} (n : @term C Node) (e : @term C OIEvent) : @prop C :=
+  ((occ <- e <- Fois) <= (@Const _ Nat 1) /\
+    alwaysp^: (Fn = n /\ self -> ~(Atom (mem <- e <- Fois))) /\
+    alwaysf^: (Fn = n /\ self -> ~(Atom (mem <- e <- Fois)))) =>:
+  (on: n, ev: [], Indication, EventOI <- e) =>:
+  ((alwaysp^: ~(on: n, ev: [], Indication, EventOI <- e)) /\
+    (alwaysf^: ~(on: n, ev: [], Indication, EventOI <- e))).
+
+End TLC.
+
+(* Constructs a list of constant terms from a sequence of values *)
+Fixpoint seq_to_term {C} t (xs : seq (@denote_type C t)) :=
+  match xs with
+  | nil => TLC.nil
+  | x :: xs' => App (App TLC.cons (@Const C t x)) (seq_to_term xs')
+  end.
