tlc/assert/prop.v
@@ -1,0 +1,277 @@
+From mathcomp.ssreflect
+Require Import ssreflect eqtype ssrbool seq.
+From tlc.utility
+Require Import seq.
+From tlc.comp
+Require Import component.
+From tlc.assert
+Require Import scope type rigid_var term atom.
+
+Set Implicit Arguments.
+Unset Strict Implicit.
+Unset Printing Implicit Defensive.
+
+Inductive prop {C} : Type :=
+| Atom (a : @atom C)
+| Conj (A1 A2 : prop)
+| Neg (A : prop)
+| Always {t} (x : @rigid_var C t) (A : prop)
+| AlwaysF' (A : prop)
+| AlwaysP' (A : prop)
+| ExistsF' (A : prop)
+| ExistsP' (A : prop)
+| Next (A : prop)
+| Self (A : prop).
+
+Bind Scope tlc_core_scope with prop.
+
+Coercion Atom : atom >-> prop.
+
+(* Basic notation for building propositions *)
+Notation "A1 /\ A2" :=
+  (Conj A1 A2)
+  (at level 80, right associativity) : tlc_core_scope.
+Notation "~ A" :=
+  (Neg A)
+  (at level 75, right associativity) : tlc_core_scope.
+Notation "'always:' x , A" :=
+  (@Always _ _ x A)
+  (at level 65, right associativity) : tlc_core_scope.
+Notation "'alwaysf^:' A" :=
+  (AlwaysF' A)
+  (at level 65, right associativity) : tlc_core_scope.
+Notation "'alwaysp^:' A" :=
+  (AlwaysP' A)
+  (at level 65, right associativity) : tlc_core_scope.
+Notation "'existsf^:' A" :=
+  (ExistsF' A)
+  (at level 65, right associativity) : tlc_core_scope.
+Notation "'existsp^:' A" :=
+  (ExistsP' A)
+  (at level 65, right associativity) : tlc_core_scope.
+Notation "'next:' A" :=
+  (Next A)
+  (at level 65, right associativity) : tlc_core_scope.
+Notation "'self:' A" :=
+  (Self A)
+  (at level 65, right associativity) : tlc_core_scope.
+
+(* Syntactic sugar *)
+Definition Disj {C} (A1 A2 : @prop C) : @prop C :=
+  ~(~A1 /\ ~A2).
+Notation "A1 \/ A2" :=
+  (Disj A1 A2)
+  (at level 85, right associativity) : tlc_core_scope.
+
+Definition Impl {C} (A1 A2 : @prop C) : @prop C :=
+  ~A1 \/ A2.
+Notation "A1 -> A2" :=
+  (Impl A1 A2)
+  (at level 99, right associativity, A2 at level 200) : tlc_core_scope.
+
+Definition Bicond {C} (A1 A2 : @prop C) : @prop C :=
+  A1 -> A2 \/ A2 -> A1.
+Notation "A1 <-> A2" :=
+  (Bicond A1 A2)
+  (at level 95, no associativity) : tlc_core_scope.
+
+Definition Exists {C t} (x : rigid_var t) (A : @prop C) : @prop C :=
+  ~always: x, ~A.
+Notation "'exists:' x , A" :=
+  (@Exists _ _ x A)
+  (at level 65, right associativity) : tlc_core_scope.
+
+Definition AlwaysF {C} (A : @prop C) : @prop C :=
+  A \/ alwaysf^: A.
+Notation "'alwaysf:' A" :=
+  (AlwaysF A)
+  (at level 65, right associativity) : tlc_core_scope.
+
+Definition AlwaysP {C} (A : @prop C) : @prop C :=
+  A \/ alwaysp^: A.
+Notation "'alwaysp:' A" :=
+  (AlwaysP A)
+  (at level 65, right associativity) : tlc_core_scope.
+
+Definition ExistsF {C} (A : @prop C) : @prop C :=
+  A \/ existsf^: A.
+Notation "'existsf:' A" :=
+  (ExistsF A)
+  (at level 65, right associativity) : tlc_core_scope.
+
+Definition ExistsP {C} (A : @prop C) : @prop C :=
+  A \/ existsp^: A.
+Notation "'existsp:' A" :=
+  (ExistsP A)
+  (at level 65, right associativity) : tlc_core_scope.
+
+Definition StrongImpl {C} (A1 A2 : @prop C) : @prop C :=
+  (alwaysf: A1) -> A2.
+Notation "A1 =>: A2" :=
+  (StrongImpl A1 A2)
+  (at level 98, right associativity) : tlc_core_scope.
+  
+Definition StrongBicond {C} (A1 A2 : @prop C) : @prop C :=
+  ((alwaysf: A1) -> A2) /\
+  ((alwaysf: A2) -> A1).
+Notation "A1 <=>: A2" :=
+  (StrongBicond A1 A2)
+  (at level 98, right associativity) : tlc_core_scope.
+
+Definition LeadsTo {C} (A1 A2 : @prop C) : @prop C :=
+  (alwaysf: A1) -> (existsf: A2).
+Notation "A1 ~> A2" :=
+  (LeadsTo A1 A2)
+  (at level 97, right associativity) : tlc_core_scope.
+
+Definition PrecBy {C} (A1 A2 : @prop C) : @prop C :=
+  (alwaysf: A1) -> (existsp: A2).
+Notation "A1 <~ A2" :=
+  (PrecBy A1 A2)
+  (at level 97, right associativity) : tlc_core_scope.
+
+(* Extracts the types of rigid variable used in a prop *)
+Fixpoint prop_var_types {C} (A : @prop C) :=
+  match A with
+  | Atom a => term_var_types a
+  | Conj A1 A2 => union (prop_var_types A1) (prop_var_types A2)
+  | Neg A0 => prop_var_types A0
+  | Always _ _ A0 => prop_var_types A0
+  | AlwaysF' A0 => prop_var_types A0
+  | AlwaysP' A0 => prop_var_types A0
+  | ExistsF' A0 => prop_var_types A0
+  | ExistsP' A0 => prop_var_types A0
+  | Next A0 => prop_var_types A0
+  | Self A0 => prop_var_types A0
+  end.
+
+(* Extracts the free rigid variables used in a prop *)
+Fixpoint prop_free_vars {C} (A : @prop C) (t : type) : seq (@rigid_var C t).
+  inversion A.
+  - (* Atom *)
+    apply (@term_vars _ _ a t).
+  - (* Conj *)
+    specialize (prop_free_vars _ A1 t) as s1.
+    specialize (prop_free_vars _ A2 t) as s2.
+    apply (union s1 s2).
+  - (* Neg *)
+    apply (prop_free_vars _ A0 t).
+  - (* Always *)
+    specialize (prop_free_vars _ A0 t) as s0.
+    case Ht: (t == t0); move/eqP: Ht => Ht.
+    - (* t = t0 *)
+      subst t0.
+      apply (rem x s0).
+    - (* t <> t0 *)
+      apply s0.
+  - (* AlwaysF' *)
+    apply (prop_free_vars _ A0 t).
+  - (* AlwaysP' *)
+    apply (prop_free_vars _ A0 t).
+  - (* ExistsF' *)
+    apply (prop_free_vars _ A0 t).
+  - (* ExistsP' *)
+    apply (prop_free_vars _ A0 t).
+  - (* Next *)
+    apply (prop_free_vars _ A0 t).
+  - (* Self *)
+    apply (prop_free_vars _ A0 t).
+Defined.
+
+(* Extracts the rigid variables used in a term *)
+Fixpoint prop_vars {C} (A : @prop C) (t : type) :=
+  match A with
+  | Atom a => term_vars a t
+  | Conj A1 A2 => union (prop_vars A1 t) (prop_vars A2 t)
+  | Neg A0 => prop_vars A0 t
+  | Always _ _ A0 => prop_vars A0 t
+  | AlwaysF' A0 => prop_vars A0 t
+  | AlwaysP' A0 => prop_vars A0 t
+  | ExistsF' A0 => prop_vars A0 t
+  | ExistsP' A0 => prop_vars A0 t
+  | Next A0 => prop_vars A0 t
+  | Self A0 => prop_vars A0 t
+  end.
+
+(* Extracts the bound rigid variables used in a term *)
+Definition prop_bound_vars {C} (A : @prop C) (t : type) :=
+  filter (fun x => x \notin prop_free_vars A t) (prop_vars A t).
+
+(* Generalizes a prop by universally quantifying all free variables *)
+Definition generalize_prop {C} (A : @prop C) :=
+  foldr (fun t A => foldr Always A (prop_free_vars A t)) A (prop_var_types A).
+
+Definition always_subst {C tx}
+(prop_subst : (forall t, @substitution C t) -> @prop C)
+(s : forall t, @substitution C t)
+(x : @rigid_var C tx) (A : @prop C) : @prop C.
+
+  have x' : rigid_var tx.
+    have p (y : rigid_var tx) : bool.
+      have e : term tx.
+        case (s _ y) => [e' | ].
+        - (* Some e' *)
+          by assumption.
+        - (* None *)
+          by exact: (Rigid y).
+      pose es := (term_vars e tx).
+      by exact: (x \in es).
+    case (has p (filter (fun y => y != x) (prop_free_vars A tx))).
+    - (* has *)
+      have s' : forall t, @rigid_var C t -> option (@term C t).
+      move=> ty; case H : (ty == tx); move/eqP: H => H.
+      - (* ty == tx *)
+        subst ty; move=> y; case (y == x).
+        - (* y == x *)
+          by exact: (Some (Rigid x)).
+        - (* y != x *)
+          by exact: (s _ y).
+      - (* ty != tx *)
+        move=> y; by exact: (s _ y).
+      by exact: fresh_rigid_var (prop_free_vars (prop_subst s') tx).
+    - (* doesn't *)
+      by exact: x.
+
+  (* Substitution to apply to the proposition A *)
+  have s' : forall t, @rigid_var C t -> option (@term C t).
+  move=> ty; case H : (ty == tx); move/eqP: H => H.
+  - (* ty == tx *)
+    subst ty; move=> y; case (y == x).
+    - (* y == x *)
+      by exact: (Some (Rigid x')).
+    - (* y != x *)
+      by exact: (s _ y).
+  - (* ty != tx *)
+    move=> y; by exact: (s _ y).
+
+  by exact: (Always x' (prop_subst s')).
+Defined.
+
+(* Substitution of terms in place of rigid variables *)
+Fixpoint prop_subst {C} (s : forall t, @substitution C t) (A : @prop C)
+: @prop C.
+  inversion A.
+  - (* Atom *)
+    exact: (Atom (term_subst s a)).
+  - (* Conj *)
+    exact: (Conj (prop_subst _ s A1) (prop_subst _ s A2)).
+  - (* Neg *)
+    exact: (Neg (prop_subst _ s A0)).
+  - (* Always *)
+    (* This is a hack; A0 is already applied to prop_subst to satisfy the
+       fixpoint decreasing argument requirements.  However, always_subst still
+       needs A0 to substitute over *)
+    apply (always_subst (fun s => prop_subst C s A0) s x A0).
+  - (* AlwaysF' *)
+    exact: (AlwaysF' (prop_subst _ s A0)).
+  - (* AlwaysP' *)
+    exact: (AlwaysP' (prop_subst _ s A0)).
+  - (* ExistsF' *)
+    exact: (ExistsF' (prop_subst _ s A0)).
+  - (* ExistsP' *)
+    exact: (ExistsP' (prop_subst _ s A0)).
+  - (* Next *)
+    exact: (Next (prop_subst _ s A0)).
+  - (* Self *)
+    exact: (Self (prop_subst _ s A0)).
+Defined.
