tlc/assert/rigid_var.v
@@ -1,0 +1,55 @@
+From mathcomp.ssreflect
+Require Import ssreflect eqtype ssrbool ssrnat seq path.
+From tlc.utility
+Require Import indeq.
+From tlc.assert
+Require Import type.
+From tlc.comp
+Require Import component.
+
+Set Implicit Arguments.
+Unset Strict Implicit.
+Unset Printing Implicit Defensive.
+
+(* Named and typed rigid variables in the assertion language *)
+Inductive rigid_var {C} : @type C -> Type :=
+| RigidVar t (n : nat) : rigid_var t.
+
+(* Equality *)
+Section eq.
+
+  Definition rigid_var_eq {C t} (x x' : @rigid_var C t) :=
+    match x, x' with
+    | RigidVar _ n, RigidVar _ n' => n == n'
+    end.
+
+  Lemma rigid_var_eqP {C t} : Equality.axiom (@rigid_var_eq C t).
+  Proof.
+    case=> ? n; case=> ? n'; indeq_auto.
+    - (* RigidVar *) by indeq n n'.
+  Qed.
+
+  Canonical rigid_var_eqMixin {C t} :=
+    EqMixin (@rigid_var_eqP C t).
+  Canonical rigid_var_eqType {C t} :=
+    Eval hnf in EqType (@rigid_var C t) (@rigid_var_eqMixin C t).
+
+End eq.
+
+(* Extracts the name of a rigid variable *)
+Definition unwrap_rigid_var {C t} (x : @rigid_var C t) :=
+  match x with
+  | RigidVar _ s => s
+  end.
+
+(* Generating fresh rigid variables *)
+Definition fresh_rigid_var {C t} (xs : seq (@rigid_var C t)) :=
+  let: ns := undup [seq unwrap_rigid_var x | x <- xs] in
+  let: ns' := sort gtn ns in
+  let: n' := head 0 ns' in
+  @RigidVar C t n'.
+Lemma fresh_rigid_var_correct {C t} (xs : seq (@rigid_var C t)) :
+  ~fresh_rigid_var xs \in xs.
+Proof.
+  (* TODO *)
+Admitted.
