tlc/assert/top_inv.v
@@ -1,0 +1,13 @@
+From mathcomp.ssreflect
+Require Import ssreflect.
+From tlc.assert
+Require Import prop top_prop.
+
+Set Implicit Arguments.
+Unset Strict Implicit.
+Unset Printing Implicit Defensive.
+
+Inductive top_inv {C} : @prop C -> Type :=
+| TI A :
+  top_prop A ->
+  top_inv (AlwaysF A).
