tlc/assert/top_prop.v
@@ -1,0 +1,47 @@
+From mathcomp.ssreflect
+Require Import ssreflect.
+From tlc.assert
+Require Import rigid_var term prop lib interleavable_prop.
+
+Set Implicit Arguments.
+Unset Strict Implicit.
+Unset Printing Implicit Defensive.
+
+Inductive top_prop {C} : @prop C -> Type :=
+| TACorrect t :
+  top_prop (Atom (App TLC.correct t))
+| TARequestEv n e :
+  top_prop (TLC.On n (TLC.Ev TLC.nil TLC.Request e))
+| TAIndicationEv n e i :
+  top_prop (TLC.On n (TLC.Ev (App (App TLC.cons i) TLC.nil) TLC.Indication e))
+| TAPeriodicEv n e :
+  top_prop (TLC.On n (TLC.Ev TLC.nil TLC.Periodic e))
+| TAConj A1 A2 :
+  top_prop A1 ->
+  top_prop A2 ->
+  top_prop (Conj A1 A2)
+| TANeg A0 :
+  top_prop A0 ->
+  top_prop (Neg A0)
+| TAAlways t (x : rigid_var t) A0 :
+  top_prop A0 ->
+  top_prop (Always x A0)
+| TAAlwaysF' A0 :
+  top_prop A0 ->
+  top_prop (AlwaysF' A0)
+| TAAlwaysP' A0 :
+  top_prop A0 ->
+  top_prop (AlwaysP' A0)
+| TAExistsF' A0 :
+  top_prop A0 ->
+  top_prop (ExistsF' A0)
+| TAExistsP' A0 :
+  top_prop A0 ->
+  top_prop (ExistsP' A0).
+
+Lemma top_prop_is_interleavable {C} A (TA : @top_prop C A) :
+  interleavable_prop A.
+Proof.
+  elim: TA; try by constructor;
+  try by (rewrite /TLC.On /TLC.Ev /TLC.Eq; repeat constructor).
+Qed.
