tlc/assert/type.v
@@ -1,0 +1,203 @@
+From mathcomp.ssreflect
+Require Import ssreflect eqtype ssrbool ssrnat seq fintype.
+From tlc.utility
+Require Import indeq seq func variant lemmas.
+From tlc.comp
+Require Import p_event component.
+From tlc.assert
+Require Import scope orientation.
+
+Set Implicit Arguments.
+Unset Strict Implicit.
+Unset Printing Implicit Defensive.
+
+(* Types of terms in the assertion language *)
+Inductive type {C : component} : Type :=
+| Unit
+| Func (t1 t2 : type)
+| Product (t1 t2 : type)
+| Sum (t1 t2 : type)
+| List (t : type)
+| Bool
+| Nat
+| Node
+| Message
+| Orientation
+| IREvent
+| OIEvent
+| OREvent' (i : 'I_(size (or_events C)))
+| IIEvent' (i : 'I_(size (ii_events C)))
+| PEvent
+| State.
+
+Bind Scope tlc_type_scope with type.
+
+(* Notations for building types *)
+Notation "x -> y" :=
+  (Func x y)
+  : tlc_type_scope.
+Notation "x * y" :=
+  (Product x y)
+  : tlc_type_scope.
+Notation "x + y" :=
+  (Sum x y)
+  : tlc_type_scope.
+Notation "[ x ]" :=
+  (List x)
+  : tlc_type_scope.
+
+(* Equality *)
+Section eq.
+
+  Fixpoint type_eq {C} (t t' : @type C) :=
+    match t, t' with
+    | Unit, Unit => true
+    | Unit, _ => false
+    | Func t1 t2, Func t1' t2' => type_eq t1 t1' && type_eq t2 t2'
+    | Func _ _, _ => false
+    | Product t1 t2, Product t1' t2' => type_eq t1 t1' && type_eq t2 t2'
+    | Product _ _, _ => false
+    | Sum t1 t2, Sum t1' t2' => type_eq t1 t1' && type_eq t2 t2'
+    | Sum _ _, _ => false
+    | List t1, List t1' => type_eq t1 t1'
+    | List _, _ => false
+    | Bool, Bool => true
+    | Nat, Nat => true
+    | Node, Node => true
+    | Message, Message => true
+    | Orientation, Orientation => true
+    | IREvent, IREvent => true
+    | OIEvent, OIEvent => true
+    | OREvent' i1, OREvent' i2 => i1 == i2
+    | OREvent' _, _ => false
+    | IIEvent' i1, IIEvent' i2 => i1 == i2
+    | IIEvent' _, _ => false
+    | State, State => true
+    | _, _ => false
+    end.
+
+  Lemma type_eqP {C} : Equality.axiom (@type_eq C).
+  Proof.
+    (* TODO *)
+  Admitted.
+
+  Canonical type_eqMixin {C} :=
+    EqMixin (@type_eqP C).
+  Canonical type_eqType {C} :=
+    Eval hnf in EqType (@type C) (@type_eqMixin C).
+
+End eq.
+
+(* Denotational semantics *)
+Section denote.
+
+  (* Maps a type to its concrete Type *)
+  Fixpoint denote_type {C} (t : @type C) : eqType :=
+    match t with
+    | Unit => [eqType of unit]
+    | Func t1 t2 => [eqType of denote_type t1 -> denote_type t2]
+    | Product t1 t2 => [eqType of prod (denote_type t1) (denote_type t2)]
+    | Sum t1 t2 => [eqType of sum (denote_type t1) (denote_type t2)]
+    | List t => [eqType of seq (denote_type t)]
+    | Bool => [eqType of bool]
+    | Nat => [eqType of nat]
+    | Node => node C
+    | Message => message C
+    | Orientation => [eqType of orientation]
+    | IREvent => ir_event C
+    | OIEvent => oi_event C
+    | OREvent' i => ith i
+    | IIEvent' i => ith i
+    | PEvent => [eqType of p_event]
+    | State => state C
+    end.
+
+  Lemma denote_unit {C} :
+    @denote_type C Unit = [eqType of unit].
+  Proof. by []. Qed.
+
+  Lemma denote_func {C} (t1 t2 : @type C) :
+    denote_type (t1 -> t2) = [eqType of denote_type t1 -> denote_type t2].
+  Proof. by []. Qed.
+
+  Lemma denote_product {C} (t1 t2 : @type C) :
+    denote_type (t1 * t2) = [eqType of prod (denote_type t1) (denote_type t2)].
+  Proof. by []. Qed.
+
+  Lemma denote_sum {C} (t1 t2 : @type C) :
+    denote_type (t1 + t2) = [eqType of sum (denote_type t1) (denote_type t2)].
+  Proof. by []. Qed.
+
+  Lemma denote_list {C} (t : @type C) :
+    denote_type [t] = [eqType of seq (denote_type t)].
+  Proof. by []. Qed.
+
+End denote.
+
+(* Parametric types *)
+Fixpoint Variant {C} (ts : seq (@type C)) : @type C :=
+  match ts with
+  | nil => Unit
+  | t :: nil => t
+  | t :: ts' => Sum t (Variant ts')
+  end.
+
+Lemma Variant_cons {C} (t : @type C) (ts : seq (@type C)) :
+  ts <> nil ->
+  Sum t (Variant ts) = Variant (t :: ts).
+Proof.
+  move=> H. case H': ts; last by [].
+  by contradiction.
+Qed.
+
+Lemma denote_variant {C} (ts : seq (@type C)) :
+  denote_type (Variant ts) = eqVariant [seq denote_type t | t <- ts].
+Proof.
+  elim Hts: ts => [ | t ts' IHts]; first by [].
+  case Hts': ts' => [ | t' ts'']; first by [].
+  rewrite -Variant_cons; last by [].
+  rewrite -eqVariant_cons; last by [].
+  by rewrite -Hts' denote_sum IHts Hts' //.
+Qed.
+
+(* Component types *)
+Definition OREvents {C} : seq (@type C) :=
+  [seq OREvent' i | i <- ord_enum (size (or_events C))].
+Definition IIEvents {C} : seq (@type C) :=
+  [seq IIEvent' i | i <- ord_enum (size (ii_events C))].
+Definition OREvent {C} : @type C :=
+  Variant OREvents.
+Definition IIEvent {C} : @type C :=
+  Variant IIEvents.
+
+Lemma denote_or_events {C} :
+  [seq @denote_type C t | t <- OREvents] = or_events C.
+Proof.
+  rewrite /OREvents /or_events map_map /denote_type.
+  by exact: map_ith_ord_enum.
+Qed.
+
+Lemma denote_ii_events {C} :
+  [seq @denote_type C t | t <- IIEvents] = ii_events C.
+Proof.
+  rewrite /IIEvents /ii_events map_map /denote_type.
+  by exact: map_ith_ord_enum.
+Qed.
+
+Lemma denote_or_event {C} : @denote_type C OREvent = or_event C.
+Proof.
+  by rewrite /OREvent /or_event denote_variant denote_or_events.
+Qed.
+
+Lemma denote_ii_event {C} : @denote_type C IIEvent = ii_event C.
+Proof.
+  by rewrite /IIEvent /ii_event denote_variant denote_ii_events.
+Qed.
+
+(* Composite types *)
+Definition Depth {C} : @type C :=
+  [Nat].
+Definition Event {C} : @type C :=
+  IREvent + OIEvent + OREvent + IIEvent + PEvent.
+Definition States {C} : @type C :=
+  Node -> State.
