tlc/comp/component.v
@@ -1,0 +1,27 @@
+From mathcomp.ssreflect
+Require Import ssreflect eqtype seq.
+From tlc.utility
+Require Import variant.
+
+Set Implicit Arguments.
+Unset Strict Implicit.
+Unset Printing Implicit Defensive.
+
+Record component :=
+  Component {
+    node : eqType;
+    message : eqType;
+    ir_event : eqType;
+    oi_event : eqType;
+    or_ii_events : seq (eqType * eqType)%type;
+    or_events := map fst or_ii_events;
+    ii_events := map snd or_ii_events;
+    or_event := eqVariant or_events;
+    ii_event := eqVariant ii_events;
+    state : eqType;
+    output := (state * (seq or_event) * (seq oi_event))%type;
+    init : node -> state;
+    request : node -> state -> ir_event -> output;
+    indication : node -> state -> ii_event -> output;
+    periodic : node -> state -> output;
+  }.
