tlc/comp/flc.v
@@ -1,155 +1,85 @@
 From mathcomp.ssreflect
 Require Import ssreflect eqtype ssrbool.
-From tlc.assert
-Require Import node_variable message_variable.
+From tlc.utility
+Require Import indeq.
 
 Set Implicit Arguments.
 Unset Strict Implicit.
 Unset Printing Implicit Defensive.
 
+(* Fair-loss link component *)
 Section flc.
 
-  Variable node : eqType.
-  Variable message : eqType.
+  Variable N : eqType. (* Node type *)
+  Variable M : eqType. (* Message type *)
 
-  (* Concrete requests *)
-  Inductive req_fl_ : Type :=
-  | Send_fl : node -> message -> req_fl_.
+  (* Requests *)
+  Section req.
 
-  (* Equality *)
-  Section req_fl__eq.
+    Inductive req_fl_ : Type :=
+    | Send_fl : N -> M -> req_fl_.
 
-    Definition eq_req_fl_ (r r' : req_fl_) :=
-      match r, r' with
-      | Send_fl n m, Send_fl n' m' => (n == n') && (m == m')
-      end.
+    (* Equality *)
+    Section eq.
 
-    Lemma eq_req_fl_P : Equality.axiom eq_req_fl_.
-    Proof.
-      case=> [n m]; case=> [n' m'];
-        rewrite /eq_req_fl_ /=; try by constructor.
-      - (* Send_fl *)
-        case Hn: (n == n');
-          [move/eqP: Hn => ?; subst n' | constructor];
-          last by case=> ?; subst n'; rewrite eqxx in Hn.
-        case Hm: (m == m');
-          [move/eqP: Hm => ?; subst m' | constructor];
-          last by case=> ?; subst m'; rewrite eqxx in Hm.
-        by constructor.
-    Qed.
+      Definition eq_req_fl_ (e e' : req_fl_) :=
+        match e, e' with
+        | Send_fl n m, Send_fl n' m' => (n == n') && (m == m')
+        end.
 
-    Canonical req_fl__eqMixin :=
-      Eval hnf in EqMixin eq_req_fl_P.
-    Canonical req_fl__eqType :=
-      Eval hnf in EqType req_fl_ req_fl__eqMixin.
+      Lemma eq_req_fl_P : Equality.axiom eq_req_fl_.
+      Proof.
+        case=> [n m]; case=> [n' m']; indeq_auto.
+        - (* Send_fl *) indeq n n'; indeq m m'; by [].
+      Qed.
+
+      Canonical req_fl__eqMixin :=
+        Eval hnf in EqMixin eq_req_fl_P.
+      Canonical req_fl__eqType :=
+        Eval hnf in EqType req_fl_ req_fl__eqMixin.
+
+    End eq.
 
     Definition req_fl := [eqType of req_fl_].
 
-  End req_fl__eq.
+  End req.
 
-  (* Assertion requests *)
-  Inductive req_fl_A_ : Type :=
-  | Send_fl_A : node_variable -> message_variable -> req_fl_A_.
+  (* Indications *)
+  Section ind.
 
-  (* Equality *)
-  Section req_fl_A__eq.
+    Inductive ind_fl_ : Type :=
+    | Deliver_fl : N -> M -> ind_fl_.
 
-    Definition eq_req_fl_A_ (r r' : req_fl_A_) :=
-      match r, r' with
-      | Send_fl_A n m, Send_fl_A n' m' => (n == n') && (m == m')
-      end.
+    (* Equality *)
+    Section eq.
 
-    Lemma eq_req_fl_A_P : Equality.axiom eq_req_fl_A_.
-    Proof.
-      case=> [n m]; case=> [n' m'];
-        rewrite /eq_req_fl_A_ /=; try by constructor.
-      - (* Send_fl_A *)
-        case Hn: (n == n');
-          [move/eqP: Hn => ?; subst n' | constructor];
-          last by case=> ?; subst n'; rewrite eqxx in Hn.
-        case Hm: (m == m');
-          [move/eqP: Hm => ?; subst m' | constructor];
-          last by case=> ?; subst m'; rewrite eqxx in Hm.
-        by constructor.
-    Qed.
+      Definition eq_ind_fl_ (e e' : ind_fl_) :=
+        match e, e' with
+        | Deliver_fl n m, Deliver_fl n' m' => (n == n') && (m == m')
+        end.
 
-    Canonical req_fl_A__eqMixin :=
-      Eval hnf in EqMixin eq_req_fl_A_P.
-    Canonical req_fl_A__eqType :=
-      Eval hnf in EqType req_fl_A_ req_fl_A__eqMixin.
+      Lemma eq_ind_fl_P : Equality.axiom eq_ind_fl_.
+      Proof.
+        case=> [n m]; case=> [n' m']; indeq_auto.
+        - (* Deliver_fl *) indeq n n'; indeq m m'; by [].
+      Qed.
 
-    Definition req_fl_A := [eqType of req_fl_A_].
+      Canonical ind_fl__eqMixin :=
+        Eval hnf in EqMixin eq_ind_fl_P.
+      Canonical ind_fl__eqType :=
+        Eval hnf in EqType ind_fl_ ind_fl__eqMixin.
 
-  End req_fl_A__eq.
-
-  (* Concrete indications *)
-  Inductive ind_fl_ : Type :=
-  | Deliver_fl : node -> message -> ind_fl_.
-
-  (* Equality *)
-  Section ind_fl__eq.
-
-    Definition eq_ind_fl_ (r r' : ind_fl_) :=
-      match r, r' with
-      | Deliver_fl n m, Deliver_fl n' m' => (n == n') && (m == m')
-      end.
-
-    Lemma eq_ind_fl_P : Equality.axiom eq_ind_fl_.
-    Proof.
-      case=> [n m]; case=> [n' m'];
-        rewrite /eq_ind_fl_ /=; try by constructor.
-      - (* Deliver_fl *)
-        case Hn: (n == n');
-          [move/eqP: Hn => ?; subst n' | constructor];
-          last by case=> ?; subst n'; rewrite eqxx in Hn.
-        case Hm: (m == m');
-          [move/eqP: Hm => ?; subst m' | constructor];
-          last by case=> ?; subst m'; rewrite eqxx in Hm.
-        by constructor.
-    Qed.
-
-    Canonical ind_fl__eqMixin :=
-      Eval hnf in EqMixin eq_ind_fl_P.
-    Canonical ind_fl__eqType :=
-      Eval hnf in EqType ind_fl_ ind_fl__eqMixin.
+    End eq.
 
     Definition ind_fl := [eqType of ind_fl_].
 
-  End ind_fl__eq.
-
-  (* Assertion indications *)
-  Inductive ind_fl_A_ : Type :=
-  | Deliver_fl_A : node_variable -> message_variable -> ind_fl_A_.
-
-  (* Equality *)
-  Section ind_fl_A__eq.
-
-    Definition eq_ind_fl_A_ (r r' : ind_fl_A_) :=
-      match r, r' with
-      | Deliver_fl_A n m, Deliver_fl_A n' m' => (n == n') && (m == m')
-      end.
-
-    Lemma eq_ind_fl_A_P : Equality.axiom eq_ind_fl_A_.
-    Proof.
-      case=> [n m]; case=> [n' m'];
-        rewrite /eq_ind_fl_A_ /=; try by constructor.
-      - (* Deliver_fl_A *)
-        case Hn: (n == n');
-          [move/eqP: Hn => ?; subst n' | constructor];
-          last by case=> ?; subst n'; rewrite eqxx in Hn.
-        case Hm: (m == m');
-          [move/eqP: Hm => ?; subst m' | constructor];
-          last by case=> ?; subst m'; rewrite eqxx in Hm.
-        by constructor.
-    Qed.
-
-    Canonical ind_fl_A__eqMixin :=
-      Eval hnf in EqMixin eq_ind_fl_A_P.
-    Canonical ind_fl_A__eqType :=
-      Eval hnf in EqType ind_fl_A_ ind_fl_A__eqMixin.
-
-    Definition ind_fl_A := [eqType of ind_fl_A_].
-
-  End ind_fl_A__eq.
+  End ind.
 
 End flc.
+
+Arguments req_fl_ {N M}.
+Arguments Send_fl {N M}.
+Arguments req_fl {N M}.
+Arguments ind_fl_ {N M}.
+Arguments Deliver_fl {N M}.
+Arguments ind_fl {N M}.
