tlc/comp/stack.v
@@ -1,25 +1,27 @@
 From mathcomp.ssreflect
 Require Import ssreflect eqtype ssrbool ssrfun seq.
 From tlc.utility
-Require Import seq.
-
-Require Import comp flc.
+Require Import mapseq.
+From tlc.comp
+Require Import component flc.
 
 Set Implicit Arguments.
 Unset Strict Implicit.
 Unset Printing Implicit Defensive.
 
+(* Stack of components *)
 Section stack.
 
-  Variable node : eqType.
-  Variable message : eqType.
-
-  Inductive stack : Type -> Type -> Type :=
-  | Stack IR OI scs :
-    comp node IR OI scs ->
-    mapseq (fun x => stack (OR x) (II x)) scs ->
+  Inductive stack {N M : eqType} : eqType -> eqType -> Type :=
+  | Stack C IR OI (Cs : seq component) :
+    node C = N ->
+    message C = M ->
+    ir_event C = IR ->
+    oi_event C = OI ->
+    or_ii_events C = [seq (ir_event x, oi_event x) | x <- Cs] ->
+    mapseq (fun x => stack (ir_event x) (oi_event x)) Cs ->
     stack IR OI
   | FairLossLink :
-    stack (req_fl node message) (ind_fl node message).
+    stack (@req_fl N M) (@ind_fl N M).
 
 End stack.
