tlc/logic/program.v
@@ -1,0 +1,54 @@
+From mathcomp.ssreflect
+Require Import ssreflect eqtype ssrbool seq fintype.
+From tlc.utility
+Require Import seq.
+From tlc.comp
+Require Import component.
+From tlc.assert
+Require Import all_assert.
+From tlc.logic
+Require Import sequent.
+
+Set Implicit Arguments.
+Unset Strict Implicit.
+Unset Printing Implicit Defensive.
+
+(* Basic rules of the program logic *)
+Section basic.
+
+  Reserved Notation "|- A"
+    (at level 80, no associativity).
+
+  Inductive program {C : component} : seq (@prop C) -> @prop C -> Prop :=
+  | PSequent X A : sequent X A -> program X A (* Program extends sequent *)
+  | PNode : |- TLC.PNode
+  | PIR (e : @term C IREvent) : |- TLC.PIR e
+  | PII (i : 'I_(size (@IIEvents C))) (e : @term C (ith i)) : |- TLC.PII e
+  | PPe : |- TLC.PPe
+  | POR (n : @term C Node) (i : 'I_(size (@OREvents C))) (e : @term C (ith i)) :
+    |- TLC.POR n e
+  | POI (n : @term C Node) (e : @term C OIEvent) : |- TLC.POI n e
+  | POR' (n : @term C Node) (i : 'I_(size (@OREvents C)))
+    (e : @term C (ith i)) : |- TLC.POR' n e
+  | POI' (n : @term C Node) (e : @term C OIEvent) : |- TLC.POI' n e
+  | PInit (n : @term C Node) : |- TLC.PInit n
+  | PPostPre (n : @term C Node) (s : @term C State) : |- TLC.PPostPre n s
+  | PSeq (n : @term C Node) : |- TLC.PSeq n
+  | PASelf : |- TLC.PASelf
+  (* TODO: PLSInv *)
+  | PCSet (n : @term C Node) : |- TLC.PCSet n
+  | PAPer (n : @term C Node) : |- TLC.PAPer n
+  (* TODO: PLFLoss *)
+  (* TODO: PLFDup *)
+  (* TODO: PLNForge *)
+  | PUniOR (n : @term C Node) (i : 'I_(size OREvents)) (e : @term C (ith i)) :
+    |- TLC.PUniOR n e
+  | PUniOI (n : @term C Node) (e : @term C OIEvent) :
+    |- TLC.PUniOI n e
+  where "|- A" := (program [::] A).
+
+End basic.
+
+Notation "X |- C , A" :=
+  (@program C X A)
+  (at level 80, no associativity).
