tlc/utility/all_utility.v
@@ -1,3 +1,7 @@
-Require Export promote.
+Require Export func.
+Require Export hseq.
+Require Export indeq.
+Require Export lemmas.
+Require Export mapseq.
 Require Export seq.
 Require Export variant.
