tlc/utility/func.v
@@ -1,0 +1,23 @@
+From mathcomp.ssreflect
+Require Import ssreflect eqtype ssrbool.
+
+Set Implicit Arguments.
+Unset Strict Implicit.
+Unset Printing Implicit Defensive.
+
+(* Equality *)
+Section eq.
+
+  Definition func_eq {d r} (f f' : d -> r) := false.
+
+  Lemma func_eqP {d r} : Equality.axiom (@func_eq d r).
+  Proof.
+    (* TODO *)
+  Admitted.
+
+  Canonical func_eqMixin {d r} :=
+    EqMixin (@func_eqP d r).
+  Canonical func_eqType {d r} :=
+    Eval hnf in EqType (d -> r) (@func_eqMixin d r).
+
+End eq.
