tlc/utility/hseq.v
@@ -1,0 +1,55 @@
+From mathcomp.ssreflect
+Require Import ssreflect seq.
+
+Set Implicit Arguments.
+Unset Strict Implicit.
+Unset Printing Implicit Defensive.
+
+Section hseq.
+
+  Variable A : Type.
+  Variable B : A -> Type.
+
+  Inductive hseq : seq A -> Type :=
+  | HNil : hseq nil
+  | HCons x xs : B x -> hseq xs -> hseq (x :: xs).
+
+  Variable x : A.
+
+  Inductive member : seq A -> Type :=
+  | HFirst xs : member (x :: xs)
+  | HNext y xs : member xs -> member (y :: xs).
+
+  Fixpoint hget xs (mxs : hseq xs) : member xs -> B x :=
+    match mxs with
+    | HNil => fun m =>
+      match m in member xs'
+      return
+        match xs' with
+        | nil => B x
+        | _ :: _ => unit
+        end
+      with
+      | HFirst _ => tt
+      | HNext _ _ _ => tt
+      end
+    | HCons _ _ y mxs' => fun m =>
+      match m in member xs'
+      return
+        match xs' with
+        | nil => Empty_set
+        | x' :: xs'' => B x' -> (member xs'' -> B x) -> B x
+        end
+      with
+      | HFirst _ => fun z _ => z
+      | HNext _ _ m' => fun _ gmxs' => gmxs' m'
+      end y (hget mxs')
+    end.
+
+End hseq.
+
+Arguments HNil [A B].
+Arguments HCons [A B x xs].
+
+Arguments HFirst [A x xs].
+Arguments HNext [A x y xs].
